DeepWiki/ReactiveSystems.lean
@@ -2,6 +2,8 @@ import DeepWiki.ReactiveSystems.LabelledTransitionSystems
 import DeepWiki.ReactiveSystems.Ccs
 import DeepWiki.ReactiveSystems.Bisimulation
 import DeepWiki.ReactiveSystems.BisimulationFixedPoint
+import DeepWiki.ReactiveSystems.Traces
+import DeepWiki.ReactiveSystems.BisimulationWeak
 
 /-! # Reactive Systems
 Autoformalization of the classic theory of reactive systems (concurrency
